some theorems that are ready for memoize

Validator/Hedge/Memoize/Memoize.lean
@@ -5,10 +5,12 @@ import Validator.Std.Hedge
 
 import Validator.Regex.Lang
 import Validator.Regex.Room
+import Validator.Regex.Memoize.Memoize
 import Validator.Hedge.Denote
 import Validator.Hedge.Grammar
 import Validator.Hedge.Room
 import Validator.Hedge.Lang
+import Validator.Hedge.Denote
 
 import Validator.Regex.Memoize
 open Regex.Memoize
@@ -24,6 +26,17 @@ namespace Hedge
 --     Regex.null (List.foldl (Grammar.Room.derive G Φ) childr children)
 --   )
 --   Regex.Room.derive nodePred r
+
+-- def Regex.Memoize.derive [Monad m] [DecidableEq σ] [Hashable σ] [MemoizeRoom m σ]
+--   (Φ: σ → Bool) (r: Regex σ): m {dr: Regex σ // dr = Regex.Room.derive Φ r } := do
+--   let ⟨symbols, hsymbols⟩ <- MemoizeRoom.enterM r
+--   let ⟨res, hres⟩ <- MemoizeRoom.leaveM ⟨r, Vector.map Φ symbols⟩
+--   let h: res = Regex.Room.derive Φ r := by
+--     unfold leave at hres
+--     simp only at hres
+--     rw [hsymbols] at hres
+--     assumption
+--   pure (Subtype.mk res h)
 
 def Grammar.Memoize.derive [DecidableEq σ] [Hashable σ] [DecidableEq α] [Hashable α] [DecidableEq φ] [Hashable φ] (G: Grammar n φ) (Φ: φ → α → Bool)
   (r: Regex (φ × Ref n)) (node: Node α): StateMemoize σ { dr: (Regex (φ × Ref n)) // dr = Grammar.Room.derive G Φ r node } :=
@@ -56,3 +69,35 @@ def Grammar.Memoize.derive [DecidableEq σ] [Hashable σ] [DecidableEq α] [Hash
       ))
   )
   Regex.Room.deriveM nodePred r
+
+--  let symbols := enter r
+--   let bools <- Vector.mapM Φ symbols
+--   pure (leave r bools)
+
+def StateMemoize.Grammar.derive.run {φ: Type} [DecidableEq φ] [Hashable φ] [DecidableEq α] [Hashable α]
+  (state: memoizeState φ) (G: Grammar n φ) (Φ: φ → α → Bool) (r: Regex (φ × Ref n)) (node: Node α): Regex (φ × Ref n) :=
+  StateMemoize.run state (Grammar.Memoize.derive G Φ r node)
+
+lemma StateMemoize.Grammar.derive.run_unfold {φ: Type} [DecidableEq φ] [Hashable φ] [DecidableEq α] [Hashable α]
+  (state: memoizeState φ) (G: Grammar n φ) (Φ: φ → α → Bool) (r: Regex (φ × Ref n)) (node: Node α):
+  (StateMemoize.Grammar.derive.run state G Φ r node) = StateMemoize.run state (Grammar.Memoize.derive G Φ r node) :=
+  rfl
+
+theorem StateMemoize.Grammar.derive.run_is_correct [DecidableEq φ] [Hashable φ] [DecidableEq α] [Hashable α]
+  (state: memoizeState φ)
+  (Φ: φ → α → Bool) (G: Grammar n φ) (r: Regex (φ × Ref n)) (node: Node α):
+  StateMemoize.Grammar.derive.run state G Φ r node = Grammar.Room.derive G Φ r node := by
+  rw [StateMemoize.Grammar.derive.run_unfold]
+  generalize StateMemoize.run state (Grammar.Memoize.derive G Φ r node) = x
+  obtain ⟨dr, hdr⟩ := x
+  simp only
+  rw [hdr]
+
+theorem StateMemoize.Grammar.derive_commutes [DecidableEq φ] [Hashable φ] [DecidableEq α] [Hashable α]
+  (state: memoizeState φ)
+  (Φ: φ → α → Prop) [DecidableRel Φ]
+  (G: Grammar n φ) (r: Regex (φ × Ref n)) (node: Node α):
+  Grammar.Rule.denote G Φ (StateMemoize.Grammar.derive.run state G (decideRel Φ) r node)
+  = Lang.derive (Grammar.Rule.denote G Φ r) node := by
+  rw [StateMemoize.Grammar.derive.run_is_correct]
+  rw [<- Grammar.Room.derive_commutes]
